# baseURI: http://www.w3.org/ns/dcat/schema
# imports: http://schema.org/
# imports: http://www.w3.org/ns/dcat
# imports: http://www.w3.org/ns/sosa/

@prefix dc: <http://purl.org/dc/elements/1.1/> .
@prefix dcat: <http://www.w3.org/ns/dcat#> .
@prefix dct: <http://purl.org/dc/terms/> .
@prefix foaf: <http://xmlns.com/foaf/0.1/> .
@prefix owl: <http://www.w3.org/2002/07/owl#> .
@prefix rdf: <http://www.w3.org/1999/02/22-rdf-syntax-ns#> .
@prefix rdfs: <http://www.w3.org/2000/01/rdf-schema#> .
@prefix schema: <http://schema.org/> .
@prefix skos: <http://www.w3.org/2004/02/skos/core#> .
@prefix sosa: <http://www.w3.org/ns/sosa/> .
@prefix xsd: <http://www.w3.org/2001/XMLSchema#> .

dc:description
  owl:equivalentProperty schema:description ;
.
dc:title
  owl:equivalentProperty schema:name ;
.
dct:description
  owl:equivalentProperty schema:description ;
.
dct:format
  owl:equivalentProperty schema:encodingFormat ;
.
dct:identifier
  owl:equivalentProperty schema:identifier ;
.
dct:issued
  owl:equivalentProperty schema:datePublished ;
.
dct:language
  owl:equivalentProperty schema:inLanguage ;
.
dct:license
  owl:equivalentProperty schema:license ;
.
dct:modified
  owl:equivalentProperty schema:dateModified ;
.
dct:publisher
  owl:equivalentProperty schema:publisher ;
.
dct:spatial
  owl:equivalentProperty schema:spatial ;
  owl:equivalentProperty schema:spatialCoverage ;
.
dct:temporal
  owl:equivalentProperty schema:datasetTimeInterval ;
  owl:equivalentProperty schema:temporal ;
  owl:equivalentProperty schema:temporalCoverage ;
.
dct:title
  owl:equivalentProperty schema:name ;
.
dcat:Catalog
  owl:equivalentClass schema:DataCatalog ;
.
dcat:DataService
  rdfs:comment "Not quite sure if a DataFeed is a data service, or a data collection. From a REST viewpoint there is no difference. But other APIs support additional queries, slices, etc which make the characterization of a service more efficient than listing all the (potentially inifinite) resources available from it." ;
  owl:equivalentClass schema:DataFeed ;
.
dcat:Dataset
  owl:equivalentClass schema:Dataset ;
.
dcat:Distribution
  owl:equivalentClass schema:DataDownload ;
.
dcat:accessURL
  schema:domainIncludes dcat:Distribution , schema:DataDownload ;
  schema:rangeIncludes rdfs:Resource , schema:Thing ;
  rdfs:subPropertyOf schema:contentUrl ;
.
dcat:byteSize
  schema:domainIncludes dcat:Distribution , schema:DataDownload ;
  schema:rangeIncludes rdfs:Literal , schema:Text;
  rdfs:subPropertyOf schema:contentSize ;
.
dcat:bytes
  schema:domainIncludes dcat:Distribution , schema:DataDownload ;
  schema:rangeIncludes xsd:integer ;
.
dcat:catalog
  schema:domainIncludes dcat:Catalog , schema:DataCatalog ;
  schema:rangeIncludes dcat:Catalog , schema:DataCatalog ;
.
dcat:contactPoint
  owl:equivalentProperty schema:contactPoint ;
.
dcat:dataDictionary
  schema:domainIncludes dcat:Dataset ;
.
dcat:dataQuality
  schema:domainIncludes dcat:Dataset ;
.
dcat:dataset
  schema:domainIncludes dcat:Catalog , schema:DataCatalog ;
  schema:rangeIncludes dcat:Dataset , schema:Dataset ;
  owl:equivalentProperty schema:dataset ;
.
dcat:distribution
  schema:domainIncludes dcat:Dataset , schema:Dataset ;
  schema:rangeIncludes dcat:Distribution , schema:DataDownload ;
  owl:equivalentProperty schema:distribution ;
.
dcat:downloadURL
  schema:domainIncludes dcat:Distribution , schema:DataDownload ;
  schema:rangeIncludes rdfs:Resource , schema:Thing ;
  rdfs:subPropertyOf schema:contentUrl ;
.
dcat:granularity
  schema:domainIncludes dcat:Dataset , schema:Dataset ;
.
dcat:keyword
  schema:domainIncludes dcat:Dataset , schema:Dataset ;
  schema:rangeIncludes rdfs:Literal , schema:Text ;
  rdfs:comment "Mapped as a sub-property of schema:keywords - dcat:keyword is singular, schema:keywords is plural" ;
  rdfs:subPropertyOf schema:keywords ;
.
dcat:landingPage
  schema:domainIncludes dcat:Dataset , schema:Dataset ;
  schema:rangeIncludes foaf:Document , schema:WebPage ;
  rdfs:subPropertyOf schema:url ;
.
dcat:mediaType
  schema:domainIncludes dcat:Distribution , schema:DataDownload ;
  schema:rangeIncludes dct:MediaTypeOrExtent ;
  owl:equivalentProperty schema:encodingFormat ;
.
dcat:record
  schema:domainIncludes dcat:Catalog , schema:DataCatalog ;
  schema:rangeIncludes dcat:CatalogRecord ;
.
dcat:service
  schema:domainIncludes dcat:Catalog , schema:DataCatalog ;
  schema:rangeIncludes dcat:DataService ;
.
dcat:size
  schema:domainIncludes dcat:Distribution , schema:DataDownload ;
.
dcat:theme
  schema:domainIncludes dcat:Dataset , schema:Dataset ;
  schema:rangeIncludes skos:Concept , schema:Class ;
  owl:equivalentProperty schema:about ;
.
dcat:themeTaxonomy
  schema:domainIncludes dcat:Catalog , schema:DataCatalog ;
  schema:rangeIncludes skos:ConceptScheme ;
.
<http://www.w3.org/ns/dcat/schema>
  rdf:type owl:Ontology ;
  dct:contributor <https://orcid.org/0000-0003-3499-8262> ;
  dct:created "2018-02-19"^^xsd:date ;
  dct:creator <http://registry.it.csiro.au/sandbox/csiro/person/Simon-Cox> ;
  dct:modified "2018-09-14"^^xsd:date ;
  rdfs:comment "<p>Based in part on Project Open Data mappings described in <a href=\"https://project-open-data.cio.gov/metadata-resources/\">https://project-open-data.cio.gov/metadata-resources/</a></p>"^^rdf:HTML ;
  rdfs:comment "<p>Based in part on SDWWG ISO 19115 - DCAT - Schema.org mapping described in <a href=\"https://www.w3.org/2015/spatial/wiki/ISO_19115_-_DCAT_-_Schema.org_mapping\">https://www.w3.org/2015/spatial/wiki/ISO_19115_-_DCAT_-_Schema.org_mapping</a></p>"^^rdf:HTML ;
  rdfs:comment "NOTE: this alignment is provisional and incomplete, and is added to the repository here to (a) support further development of the DCAT-SDO alignment (b) demonstrate the strategy of modularizing alignments and dependencies into separate RDF files." ;
  rdfs:comment "RDF graph containing alignment axioms between DCAT and schema.org" ;
  rdfs:label "DCAT-SDO alignment" ;
  rdfs:seeAlso <https://github.com/w3c/dxwg/issues/110> ;
  rdfs:seeAlso <https://project-open-data.cio.gov/metadata-resources/> ;
  rdfs:seeAlso <https://www.w3.org/2015/spatial/wiki/ISO_19115_-_DCAT_-_Schema.org_mapping> ;
  owl:imports schema: ;
  owl:imports <http://www.w3.org/ns/dcat> ;
  owl:imports sosa: ;
.
sosa:hasFeatureOfInterest
  rdfs:subPropertyOf schema:object ;
.
sosa:hasResult
  rdfs:subPropertyOf schema:result ;
.
sosa:madeByActuator
  rdfs:subPropertyOf schema:instrument ;
.
sosa:madeBySampler
  rdfs:subPropertyOf schema:instrument ;
.
sosa:madeBySensor
  rdfs:subPropertyOf schema:instrument ;
.
sosa:observedProperty
  owl:equivalentProperty schema:variableMeasured ;
.
sosa:phenomenonTime
  rdfs:subPropertyOf schema:temporalCoverage ;
.
sosa:resultTime
  rdfs:subPropertyOf schema:endTime ;
.
sosa:usedProcedure
  owl:equivalentProperty schema:measurementTechnique ;
.
foaf:Organization
  owl:equivalentClass schema:Organization ;
.
foaf:homepage
  owl:equivalentProperty schema:url ;
.
foaf:mbox
  owl:equivalentProperty schema:email ;
.
