# baseURI: http://www.w3.org/ns/dcat/prov
# imports: http://www.w3.org/ns/dcat
# imports: http://www.w3.org/ns/prov-o
# prefix: dcat-prov

@prefix dcat: <http://www.w3.org/ns/dcat#> .
@prefix dcat-prov: <http://www.w3.org/ns/dcat/prov#> .
@prefix dct: <http://purl.org/dc/terms/> .
@prefix foaf: <http://xmlns.com/foaf/0.1/> .
@prefix owl: <http://www.w3.org/2002/07/owl#> .
@prefix prov: <http://www.w3.org/ns/prov#> .
@prefix rdf: <http://www.w3.org/1999/02/22-rdf-syntax-ns#> .
@prefix rdfs: <http://www.w3.org/2000/01/rdf-schema#> .
@prefix skos: <http://www.w3.org/2004/02/skos/core#> .
@prefix xsd: <http://www.w3.org/2001/XMLSchema#> .

dct:contributor
  rdfs:subPropertyOf prov:wasAttributedTo ;
  owl:propertyChainAxiom (
      [
        rdf:type owl:ObjectProperty ;
        rdfs:range [
            rdf:type owl:Class ;
            rdfs:subClassOf prov:Attribution ;
            rdfs:subClassOf [
                rdf:type owl:Restriction ;
                owl:hasValue <http://registry.it.csiro.au/def/isotc211/CI_RoleCode/contributor> ;
                owl:onProperty dcat:hadRole ;
              ] ;
          ] ;
        rdfs:subPropertyOf prov:qualifiedAttribution ;
      ]
      prov:agent
    ) ;
.
dct:creator
  owl:propertyChainAxiom (
      [
        rdf:type owl:ObjectProperty ;
        rdfs:range [
            rdf:type owl:Class ;
            rdfs:subClassOf prov:Attribution ;
            rdfs:subClassOf [
                rdf:type owl:Restriction ;
                owl:hasValue <https://inspire.ec.europa.eu/metadata-codelist/ResponsiblePartyRole/originator> ;
                owl:onProperty dcat:hadRole ;
              ] ;
          ] ;
        rdfs:subPropertyOf prov:qualifiedAttribution ;
      ]
      prov:agent
    ) ;
.
dct:hasFormat
  rdfs:subPropertyOf prov:alternateOf ;
.
dct:isFormatOf
  rdfs:subPropertyOf prov:alternateOf ;
.
dct:isVersionOf
  rdfs:subPropertyOf prov:wasRevisionOf ;
.
dct:publisher
  rdfs:subPropertyOf prov:wasAttributedTo ;
  owl:propertyChainAxiom (
      [
        rdf:type owl:ObjectProperty ;
        rdfs:range [
            rdf:type owl:Class ;
            rdfs:subClassOf prov:Attribution ;
            rdfs:subClassOf [
                rdf:type owl:Restriction ;
                owl:hasValue <http://inspire.ec.europa.eu/metadata-codelist/ResponsiblePartyRole/publisher> ;
                owl:onProperty dcat:hadRole ;
              ] ;
          ] ;
        rdfs:subPropertyOf prov:qualifiedAttribution ;
      ]
      prov:agent
    ) ;
.
dct:references
  rdfs:subPropertyOf prov:wasDerivedFrom ;
.
dct:source
  rdfs:subPropertyOf prov:wasDerivedFrom ;
.
dcat:Catalog
  rdfs:subClassOf prov:Collection ;
  rdfs:subClassOf [
      rdf:type owl:Restriction ;
      owl:allValuesFrom dcat:Resource ;
      owl:onProperty prov:hadMember ;
    ] ;
.
dcat:CatalogRecord
  rdfs:subClassOf prov:Entity ;
  skos:editorialNote """2018-02-28 AGB: Links to requirements mentioned above in the github tracker to follow the discussions
https://github.com/w3c/dxwg/issues/71
https://github.com/w3c/dxwg/issues/66
https://github.com/w3c/dxwg/issues/76""" ;
.
dcat:Distribution
  rdfs:subClassOf prov:Entity ;
.
dcat:QualifiedRelationship
  rdf:type owl:Class ;
  rdfs:comment "An instance of dcat:QualifiedRelationship provides additional descriptions about the binary dct:relation relation from some Entity to a related Entity."@en ;
  rdfs:label "Qualified relation" ;
  prov:unqualifiedForm dct:relation ;
.
dcat:Resource
  rdfs:subClassOf prov:Entity ;
  skos:editorialNote """2018-02-28 AGB: Links to requirements mentioned above in the github tracker to follow the discussions
https://github.com/w3c/dxwg/issues/71
https://github.com/w3c/dxwg/issues/66
https://github.com/w3c/dxwg/issues/76""" ;
.
dcat:Role
  rdf:type owl:Class ;
  rdfs:label "Role" ;
  rdfs:seeAlso prov:hadRole ;
  prov:category "qualified" ;
  prov:definition "A role is the function of an entity or agent with respect to an entity."@en ;
.
dcat:catalog
  rdfs:subPropertyOf prov:hadMember ;
.
dcat:dataset
  rdfs:subPropertyOf prov:hadMember ;
.
dcat:hadRole
  rdf:type owl:ObjectProperty ;
  rdfs:comment "The _optional_ Role that an Agent or other Entity assumed in the context of an Entity."@en ;
  rdfs:domain [
      rdf:type owl:Class ;
      owl:unionOf (
          prov:Attribution
          dcat:QualifiedRelationship
        ) ;
    ] ;
  rdfs:label "had role" ;
  rdfs:range prov:Role ;
  prov:category "qualified" ;
.
dcat:qualifiedRelation
  rdf:type owl:ObjectProperty ;
  rdfs:comment "If this Entity dct:relation Entity :e, then it can qualify how it was derived using dcat:qualifiedRelation [ a dcat:QualifiedRelationship ;  prov:entity :e; :foo :bar ]."@en ;
  rdfs:domain prov:Entity ;
  rdfs:range dcat:QualifiedRelationship ;
  rdfs:subPropertyOf prov:qualifiedInfluence ;
  prov:category "qualified" ;
  prov:unqualifiedForm dct:relation ;
.
dcat:service
  rdfs:subPropertyOf prov:hadMember ;
.
<http://www.w3.org/ns/dcat/prov>
  rdf:type owl:Ontology ;
  dct:created "2018-02-19"^^xsd:date ;
  dct:creator <http://registry.it.csiro.au/sandbox/csiro/person/Simon-Cox> ;
  dct:creator <https://www.w3.org/2017/dxwg/wiki/Main_Page> ;
  rdfs:comment "NOTE: this alignment is provisional and incomplete, and is added to the repository here to (a) support further development of the DCAT-PROV alignment (b) demonstrate the strategy of modularizing alignments and dependencies into separate RDF files." ;
  rdfs:comment "RDF graph containing alignment axioms between DCAT and PROV-O" ;
  rdfs:label "DCAT-PROV alignment" ;
  rdfs:seeAlso <https://github.com/w3c/dxwg/issues/111> ;
  rdfs:seeAlso <https://github.com/w3c/dxwg/issues/128> ;
  rdfs:seeAlso <https://github.com/w3c/dxwg/issues/134> ;
  rdfs:seeAlso <https://github.com/w3c/dxwg/pull/94> ;
  owl:imports <http://www.w3.org/ns/dcat> ;
  owl:imports <http://www.w3.org/ns/prov-o> ;
.
prov:Agent
  rdfs:comment "prov:Agent is modeled as a subclass of foaf:Agent since it is the subset of agents that are involved in prov:Activity individuals" ;
  rdfs:subClassOf foaf:Agent ;
.
prov:hadMember
  rdfs:subPropertyOf dct:hasPart ;
.
<https://www.w3.org/2017/dxwg/wiki/Main_Page>
  rdf:type foaf:Agent ;
  rdfs:label "W3C Data Exchange Working Group" ;
.
