# baseURI: http://www.w3.org/ns/dcat-service
# imports: http://purl.org/dc/terms/
# imports: http://www.w3.org/2004/02/skos/core
# imports: http://www.w3.org/ns/dcat
# imports: http://www.w3.org/ns/dcat/prov
# prefix: dcat-s

@prefix dcat: <http://www.w3.org/ns/dcat#> .
@prefix dcat-s: <http://www.w3.org/ns/dcat-service#> .
@prefix dcterms: <http://purl.org/dc/terms/> .
@prefix dctype: <http://purl.org/dc/dcmitype/> .
@prefix foaf: <http://xmlns.com/foaf/0.1/> .
@prefix owl: <http://www.w3.org/2002/07/owl#> .
@prefix rdf: <http://www.w3.org/1999/02/22-rdf-syntax-ns#> .
@prefix rdfs: <http://www.w3.org/2000/01/rdf-schema#> .
@prefix skos: <http://www.w3.org/2004/02/skos/core#> .
@prefix xsd: <http://www.w3.org/2001/XMLSchema#> .

dcat:Catalog
  rdfs:subClassOf [
      rdf:type owl:Restriction ;
      owl:allValuesFrom dcat:CataloguedItem ;
      owl:onProperty dcterms:hasPart ;
    ] ;
  rdfs:subClassOf [
      rdf:type owl:Restriction ;
      owl:minCardinality "1"^^xsd:nonNegativeInteger ;
      owl:onProperty dcterms:conformsTo ;
    ] ;
.
dcat:CatalogRecord
  rdfs:subClassOf [
      rdf:type owl:Restriction ;
      owl:allValuesFrom dcat:CataloguedItem ;
      owl:onProperty foaf:primaryTopic ;
    ] ;
  rdfs:subClassOf [
      rdf:type owl:Restriction ;
      owl:cardinality "1"^^xsd:nonNegativeInteger ;
      owl:onProperty foaf:primaryTopic ;
    ] ;
.
dcat:CataloguedItem
  rdf:type owl:Class ;
  rdfs:label "Item in a DCAT Catalog" ;
.
dcat:DataDistributionService
  rdf:type owl:Class ;
  rdfs:comment "A site or end-point that provides access to datasets and distributions of datasets" ;
  rdfs:label "Data distribution service" ;
  rdfs:subClassOf dctype:Service ;
  rdfs:subClassOf dcat:Service ;
  rdfs:subClassOf [
      rdf:type owl:Restriction ;
      owl:hasValue <https://inspire.ec.europa.eu/metadata-codelist/SpatialDataServiceType/download> ;
      owl:onProperty dcterms:type ;
    ] ;
.
dcat:DataTransformationService
  rdf:type owl:Class ;
  rdfs:comment "A site or end-point that provides a service to transform datasets in some way, e.g. spatial coordinates, schematic representation, interpolation, re-sampling" ;
  rdfs:label "Other service" ;
  rdfs:subClassOf dctype:Service ;
  rdfs:subClassOf dcat:Service ;
  rdfs:subClassOf [
      rdf:type owl:Restriction ;
      owl:hasValue <https://inspire.ec.europa.eu/metadata-codelist/SpatialDataServiceType/transformation> ;
      owl:onProperty dcterms:type ;
    ] ;
.
dcat:DiscoveryService
  rdf:type owl:Class ;
  rdfs:label "Resource DIscovery Service" ;
  rdfs:subClassOf dcat:Catalog ;
  rdfs:subClassOf dcat:Service ;
  rdfs:subClassOf [
      rdf:type owl:Restriction ;
      owl:hasValue <http://inspire.ec.europa.eu/metadata-codelist/SpatialDataServiceType/discovery> ;
      owl:onProperty dcterms:type ;
    ] ;
.
dcat:Service
  rdf:type owl:Class ;
  rdfs:label "Service" ;
  rdfs:subClassOf dcat:CataloguedItem ;
  rdfs:subClassOf [
      rdf:type owl:Restriction ;
      owl:minCardinality "1"^^xsd:nonNegativeInteger ;
      owl:onProperty dcterms:conformsTo ;
    ] ;
  rdfs:subClassOf [
      rdf:type owl:Restriction ;
      owl:minCardinality "1"^^xsd:nonNegativeInteger ;
      owl:onProperty dcterms:type ;
    ] ;
.
dcat:accessService
  rdf:type owl:ObjectProperty ;
  rdfs:comment "link to DataDistributionService that can serves this data Distribution" ;
  rdfs:domain dcat:Distribution ;
  rdfs:label "data access services" ;
  rdfs:range dcat:DataDistributionService ;
.
dcat:catalog
  rdf:type owl:ObjectProperty ;
  rdfs:comment "Link from a catalog to another catalog whose contents are of interest in the context of this catalog" ;
  rdfs:domain dcat:Catalog ;
  rdfs:label "Link to catalog" ;
  rdfs:range dcat:Catalog ;
  rdfs:subPropertyOf dcterms:hasPart ;
  rdfs:subPropertyOf rdfs:member ;
.
dcat:dataset
  rdfs:subPropertyOf rdfs:member ;
.
dcat:servesDataset
  rdf:type owl:ObjectProperty ;
  rdfs:comment "Link to description of a dataset that this DataDistributionService can distribute" ;
  rdfs:domain dcat:DataDistributionService ;
  rdfs:label "serves dataset" ;
  rdfs:range dcat:Dataset ;
.
dcat:service
  rdf:type owl:ObjectProperty ;
  rdfs:comment "link to description of a service" ;
  rdfs:domain dcat:Catalog ;
  rdfs:label "has service" ;
  rdfs:range dcat:Service ;
  rdfs:subPropertyOf dcterms:hasPart ;
  rdfs:subPropertyOf rdfs:member ;
.
<http://www.w3.org/ns/dcat-service>
  rdf:type owl:Ontology ;
  owl:imports dcterms: ;
  owl:imports <http://www.w3.org/2004/02/skos/core> ;
  owl:imports <http://www.w3.org/ns/dcat> ;
  owl:imports <http://www.w3.org/ns/dcat/prov> ;
  owl:versionInfo "Created with TopBraid Composer" ;
.
