# baseURI: http://www.w3.org/ns/dcat/prov
# imports: http://www.w3.org/ns/dcat
# imports: http://www.w3.org/ns/prov-o
# prefix: dcat-prov

@prefix dcat: <http://www.w3.org/ns/dcat#> .
@prefix dcat-prov: <http://www.w3.org/ns/dcat/prov#> .
@prefix dct: <http://purl.org/dc/terms/> .
@prefix foaf: <http://xmlns.com/foaf/0.1/> .
@prefix owl: <http://www.w3.org/2002/07/owl#> .
@prefix prov: <http://www.w3.org/ns/prov#> .
@prefix rdf: <http://www.w3.org/1999/02/22-rdf-syntax-ns#> .
@prefix rdfs: <http://www.w3.org/2000/01/rdf-schema#> .
@prefix skos: <http://www.w3.org/2004/02/skos/core#> .
@prefix xsd: <http://www.w3.org/2001/XMLSchema#> .

dct:contributor
  rdfs:subPropertyOf prov:wasAttributedTo ;
.
dct:hasFormat
  rdfs:subPropertyOf prov:alternateOf ;
.
dct:isFormatOf
  rdfs:subPropertyOf prov:alternateOf ;
.
dct:isVersionOf
  rdfs:subPropertyOf prov:wasRevisionOf ;
.
dct:publisher
  rdfs:subPropertyOf prov:wasAttributedTo ;
.
dct:references
  rdfs:subPropertyOf prov:wasDerivedFrom ;
.
dct:source
  rdfs:subPropertyOf prov:wasDerivedFrom ;
.
dcat:Catalog
  rdfs:subClassOf prov:Collection ;
  rdfs:subClassOf [
      rdf:type owl:Restriction ;
      owl:allValuesFrom dcat:Resource ;
      owl:onProperty prov:hadMember ;
    ] ;
.
dcat:CatalogRecord
  rdfs:subClassOf prov:Entity ;
  skos:editorialNote """2018-02-28 AGB: Links to requirements mentioned above in the github tracker to follow the discussions
https://github.com/w3c/dxwg/issues/71
https://github.com/w3c/dxwg/issues/66
https://github.com/w3c/dxwg/issues/76""" ;
.
dcat:Distribution
  rdfs:subClassOf prov:Entity ;
.
dcat:Resource
  rdfs:subClassOf prov:Entity ;
  skos:editorialNote """2018-02-28 AGB: Links to requirements mentioned above in the github tracker to follow the discussions
https://github.com/w3c/dxwg/issues/71
https://github.com/w3c/dxwg/issues/66
https://github.com/w3c/dxwg/issues/76""" ;
.
dcat:catalog
  rdfs:subPropertyOf prov:hadMember ;
.
dcat:dataset
  rdfs:subPropertyOf prov:hadMember ;
.
dcat:service
  rdfs:subPropertyOf prov:hadMember ;
.
<http://www.w3.org/ns/dcat/prov>
  rdf:type owl:Ontology ;
  dct:created "2018-02-19"^^xsd:date ;
  dct:creator <http://orcid.org/0000-0002-3884-3420> ;
  dct:creator <https://www.w3.org/2017/dxwg/wiki/Main_Page> ;
  rdfs:comment "NOTE: this alignment is provisional and incomplete, and is added to the repository here to (a) support further development of the DCAT-PROV alignment (b) demonstrate the strategy of modularizing alignments and dependencies into separate RDF files." ;
  rdfs:comment "RDF graph containing alignment axioms between DCAT and PROV-O" ;
  rdfs:label "DCAT-PROV alignment" ;
  rdfs:seeAlso <https://github.com/w3c/dxwg/issues/111> ;
  rdfs:seeAlso <https://github.com/w3c/dxwg/issues/128> ;
  rdfs:seeAlso <https://github.com/w3c/dxwg/issues/134> ;
  rdfs:seeAlso <https://github.com/w3c/dxwg/issues?q=label%3Aprovenance> ;
  rdfs:seeAlso <https://github.com/w3c/dxwg/pull/94> ;
  rdfs:seeAlso <https://github.com/w3c/dxwg/wiki/Provenance-patterns> ;
  rdfs:seeAlso <https://github.com/w3c/dxwg/wiki/Qualified-relations> ;
  rdfs:seeAlso <https://www.w3.org/TR/prov-dc/> ;
  owl:imports <http://www.w3.org/ns/dcat> ;
  owl:imports <http://www.w3.org/ns/prov-o> ;
  skos:editorialNote "NOTE: Currently includes the apparatus required for Qualified Relations, since some of these build on elements from PROV-O" ;
  skos:editorialNote "NOTE: Includes some alignments from Dublin Core to PROV Mapping https://www.w3.org/TR/prov-dc/" ;
.
prov:Agent
  rdfs:comment "prov:Agent is modeled as a subclass of foaf:Agent since it is the subset of agents that are involved in prov:Activity individuals" ;
  rdfs:subClassOf foaf:Agent ;
.
prov:hadMember
  rdfs:subPropertyOf dct:hasPart ;
.
<https://www.w3.org/2017/dxwg/wiki/Main_Page>
  rdf:type foaf:Agent ;
  rdfs:label "W3C Data Exchange Working Group" ;
.
