@prefix dc: <http://purl.org/dc/elements/1.1/> .
@prefix dct: <http://purl.org/dc/terms/> .
@prefix owl: <http://www.w3.org/2002/07/owl#> .
@prefix rdf: <http://www.w3.org/1999/02/22-rdf-syntax-ns#> .
@prefix rdfs: <http://www.w3.org/2000/01/rdf-schema#> .
@prefix skos: <http://www.w3.org/2004/02/skos/core#> .
@prefix xsd: <http://www.w3.org/2001/XMLSchema#> .
@prefix foaf: <http://xmlns.com/foaf/0.1/> .
@prefix prov: <http://www.w3.org/ns/prov#> .


@prefix dcat: <http://www.w3.org/ns/dcat#> .
@prefix prof: <http://www.w3.org/ns/dcat/profile#> .


# axioms repeated/included here unchanged, for convenience
dct:conformsTo
	a rdf:Property ;
	rdfs:comment "An established standard to which the described resource conforms."@en ;
    rdfs:isDefinedBy <http://purl.org/dc/terms/> ;
    rdfs:label "Conforms To"@en ;
    rdfs:range dct:Standard ;
	rdfs:subPropertyOf <http://purl.org/dc/elements/1.1/relation>, dct:relation ;
. 

<http://www.w3.org/ns/dcat/profile>
  rdf:type owl:Ontology ;
  dc:creator "Rob Atkinson" ;
  dc:description  "This is an RDF/OWL Ontology for describing relationships between Specifications, implementing profiles and supporting artefacts" ;
  rdfs:comment "This model provides a canonical vocabulary for describing profiling relationships between http://dublincore.org/2012/06/14/dcterms#Standard entities and attachment of resources defining additional constraints"@en ;
  dct:modified "2018-02-16" ;
.

prof:Profile
  rdf:type owl:Class ;
  rdf:subClassOf dct:Standard, skos:Concept ;
  rdfs:label "Implementation Profile" ;
  dc:description "A named set of constraints on one or more identified base specifications, including the identification of any implementing subclasses of datatypes, semantic interpretations, vocabularies, options and parameters of those base specifications necessary to accomplish a particular function."@en;
  dc:source <https://www.w3.org/2017/dxwg/wiki/ProfileContext> ;
  rdfs:comment "Profile is modelled as a skos:Concept to explicitly support the notion of profiles organised as classification taxonomies. skos:broader/narrower and broaderTransitive properties may be used ";
.

prof:BaseSpecification
  rdf:type owl:Class ;
  rdfs:subClassOf prof:Profile ;
  rdfs:label "Base Specification" ;
  dc:description "A specification that defines all implementation constraints, without applying constraints on usage of another specification"@en;
  rdfs:comment "This may not be a useful class, but documents that any specification can be regarded as a trivial profile, so applications only need to be concerned with Profile conformance"@en;
  rdfs:subClassOf [
      rdf:type owl:Restriction ;
      owl:maxCardinality "0"^^xsd:nonNegativeInteger ;
      owl:onProperty prof:profileOf ;
    ] ;
.

prof:profileOf
  rdf:type owl:ObjectProperty ;
  rdfs:label "profiles" ;
  dc:description "a base specification a Profile conforms to"@en ;
  rdfs:comment "The semantics of the rdfs:Range means that any resource treated as a base specification can be regarded as a Profile (i.e. may be any specification with an empty set of additional constraints)"@en ;
  rdfs:range prof:Profile ;
  rdfs:domain prof:Profile ;
  owl:inverseOf prof:hasProfile ;
.

prof:hasProfile
  rdf:type owl:ObjectProperty ;
  rdfs:label "hasProfile" ;
  dc:description "known profiles of a specification"@en ;
  rdfs:range prof:Profile ;
  owl:inverseOf prof:profileOf ;
.

prof:token
  rdf:type owl:DatatypeProperty ;
  rdfs:label "short name" ;
  dc:description "A token identifying this profile for use in APIs"@en ;
  rdfs:comment "Avoids need for a global registry - APIs may need to have some concept of a namespace for tokens to disambiguate - but should tokens be versioned? Should we just use skos:notation? "@en ;
  rdfs:range prof:Profile ;
  rdfs:domain xsd:token ;
.


prof:resource
  rdf:type owl:ObjectProperty ;
  rdfs:label "Implementing Resource"@en ;
  dc:description "URI link to resource"@en ;
  rdfs:range prof:ImplResourceDesc ;
.

prof:ImplResourceDesc
  rdf:type owl:Class ;
  rdfs:label "Implementation Resource Descriptor"@en ;
  dc:description "A resource that defines implementing rules for a profile. Must indicate the purpose (dct:type) and the formalism (dct:format) used to allow machine mediation of such rules."@en ;
  rdfs:subClassOf [
      rdf:type owl:Restriction ;
      owl:cardinality "1"^^xsd:nonNegativeInteger ;
      owl:onProperty prof:resourceRole ;
    ] ;

  rdfs:subClassOf [
      rdf:type owl:Restriction ;
      owl:cardinality "1"^^xsd:nonNegativeInteger ;
      owl:onProperty prof:resource ;
    ] ;
  rdfs:subClassOf [
      rdf:type owl:Restriction ;
      owl:minCardinality "1"^^xsd:nonNegativeInteger ;
      owl:onProperty dct:format ;
    ] ;
.

prof:resourceRole a owl:ObjectProperty ;
	rdfs:label "Functional role of implementation resource" ;
	rdfs:comment "Not sure if this should be bound to a specific vocabulary - so a couple of examples provided here" ;
	rdfs:domain prof:ImplResourceDesc ;
  	rdfs:range skos:Concept ;
.

prof:resourceType a owl:ObjectProperty ;
	rdfs:label "Type (model) of implementation resource" ;
	rdfs:comment "e.g. SHACL" ;
	rdfs:domain prof:ImplResourceDesc ;
  	rdfs:range skos:Concept ;
.

prof:ImplResourceType a owl:Class ;
	rdfs:subClassOf skos:Concept ;
.


prof:resourceRoles  a skos:ConceptScheme ;
	skos:note "Suggested subset of possible roles a resource may play with regard to a profile"@en;
.

prof:fullConstraints a prof:ImplResourceType;
	skos:prefLabel "Complete set of constraints for a profile"@en;
	rdfs:comment "Note that this means a full set of constraints within the scope of the resource type - e.g. everything that can be tested by SHACL"@en ;
	skos:topConceptOf prof:resourceRoles ;
.

prof:conformanceTest a prof:ImplResourceType;
	skos:prefLabel "Constraints specifying a conformance Test "@en;
	rdfs:comment "A normative conformance test - may also be a a fullConstraints or partConstraints resource."@en ;
	skos:topConceptOf prof:resourceRoles ;
.

prof:partConstraints a prof:ImplResourceType;
	skos:prefLabel "Partial set of constraints for a profile"@en;
	skos:topConceptOf prof:resourceRoles ;
.

prof:guidance a prof:ImplResourceType;
	skos:prefLabel "Guidance notes of profile"@en;
	skos:topConceptOf prof:resourceRoles ;
.

prof:FullConstraintSet rdfs:subClassOf prof:ImplResourceType ;
	a skos:Concept ;
.